Factored out some proofs that rely only on base being powers of two, and defined conversion between two such bases. This will allow conversion between the pseudomersenne base representation and the wire format. Also relocated some lemmas to Util.

src/ModularArithmetic/ModularBaseSystem.v
@@ -8,6 +8,7 @@ Require Import Crypto.ModularArithmetic.PseudoMersenneBaseParamProofs.
 Require Import Crypto.ModularArithmetic.ExtendedBaseVector.
 Require Import Crypto.Tactics.VerdiTactics.
 Require Import Crypto.Util.Notations.
+Require Import Crypto.ModularArithmetic.Pow2Base.
 Local Open Scope Z_scope.
 
 Section PseudoMersenneBase.
@@ -19,16 +20,8 @@ Section PseudoMersenneBase.
   Local Notation "u ~= x" := (rep u x).
   Local Hint Unfold rep.
 
-  (* i is current index, counts down *)
-  Fixpoint encode' z i : digits :=
-    match i with
-    | O => nil
-    | S i' => let lw := sum_firstn limb_widths in
-       encode' z i' ++ (Z.shiftr (Z.land z (Z.ones (lw i))) (lw i')) :: nil
-    end.
-
   (* max must be greater than input; this is used to truncate last digit *)
-  Definition encode (x : F modulus) := encode' x (length base).
+  Definition encode (x : F modulus) := encodeZ limb_widths x.
 
   (* Converts from length of extended base to length of base by reduction modulo M.*)
   Definition reduce (us : digits) : digits :=
@@ -109,15 +102,6 @@ Section Canonicalization.
 
   (* compute at compile time *)
   Definition modulus_digits := modulus_digits' (length base - 1).
-
-  Fixpoint map2 {A B C} (f : A -> B -> C) (la : list A) (lb : list B) : list C :=
-    match la with
-    | nil => nil
-    | a :: la' => match lb with
-                  | nil => nil
-                  | b :: lb' => f a b :: map2 f la' lb'
-                  end
-    end.
 
   Definition and_term us := if isFull us then max_ones else 0.
 
